src/Lean/Meta/Tactic/Simp/BuiltinSimprocs/BitVec.lean
@@ -167,8 +167,8 @@ builtin_dsimproc [simp, seval] reduceGetMsb (getMsbD _ _) := reduceGetBit ``getM
 /-- Simplification procedure for `clz` (count leading zeros) on `BitVec`. -/
 builtin_dsimproc [simp, seval] reduceClz (clz _) := reduceUnary ``BitVec.clz 2 BitVec.clz
 
-/-- Simplification procedure for `popCount` (population count) on `BitVec`. -/
-builtin_dsimproc [simp, seval] reducePopCount (popCount _) := reduceUnary ``BitVec.popCount 2 BitVec.popCount
+/-- Simplification procedure for `cpop` (population count) on `BitVec`. -/
+builtin_dsimproc [simp, seval] reduceCpop (cpop _) := reduceUnary ``BitVec.cpop 2 BitVec.cpop
 
 /-- Simplification procedure for `getElem`  on `BitVec`. -/
 builtin_dsimproc [simp, seval] reduceGetElem ((_ : BitVec _)[_]) := fun e => do
