src/Std/Tactic/BVDecide/Bitblast/BVExpr/Circuit/Lemmas/Expr.lean
@@ -17,7 +17,7 @@ public import Std.Tactic.BVDecide.Bitblast.BVExpr.Circuit.Lemmas.Operations.Mul
 public import Std.Tactic.BVDecide.Bitblast.BVExpr.Circuit.Lemmas.Operations.Umod
 public import Std.Tactic.BVDecide.Bitblast.BVExpr.Circuit.Lemmas.Operations.Reverse
 public import Std.Tactic.BVDecide.Bitblast.BVExpr.Circuit.Lemmas.Operations.Clz
-public import Std.Tactic.BVDecide.Bitblast.BVExpr.Circuit.Lemmas.Operations.PopCount
+public import Std.Tactic.BVDecide.Bitblast.BVExpr.Circuit.Lemmas.Operations.Cpop
 public import Std.Tactic.BVDecide.Bitblast.BVExpr.Circuit.Impl.Expr
 import Init.ByCases
 import Init.Data.Nat.Linear
